src/Language/PlutusIR/Semantics/SemanticEquivalence/CompatibilityLemmas.v
@@ -1,0 +1,2 @@
+Require Export PlutusCert.Language.PlutusIR.Semantics.SemanticEquivalence.CompatibilityLemmas.Apply.
+Require Export PlutusCert.Language.PlutusIR.Semantics.SemanticEquivalence.CompatibilityLemmas.Constant.
