src/Language/PlutusIR/Semantics/SemanticEquivalence/CompatibilityLemmas/Constant.v
@@ -1,0 +1,26 @@
+Require Import PlutusCert.Language.PlutusIR.
+Import NamedTerm.
+Require Import PlutusCert.Language.PlutusIR.Semantics.Dynamic.
+Require Import PlutusCert.Language.PlutusIR.Semantics.Static.
+Require Import PlutusCert.Language.PlutusIR.Semantics.Static.Implementations.Named.
+Require Import PlutusCert.Language.PlutusIR.Semantics.SemanticEquivalence.Def.
+
+Require Import Arith.
+
+
+Lemma RC_compatibility_Constant : forall k u a,
+    RC k (Ty_Builtin (Some (TypeIn u))) (Constant (Some (ValueOf u a))) (Constant (Some (ValueOf u a))).
+Proof.
+  intros k u a.
+
+  split. { apply T_Constant. } 
+  split. { apply T_Constant. }
+
+  intros j Hlt__j e_f Hev__e.
+
+  exists e_f, j. split; auto.
+
+  intros. subst.
+  inversion Hev__e. subst.
+  reflexivity.
+Qed.
